add TNat with finished proofs for all except subst_ind_correct

project/Main.v
@@ -11,7 +11,8 @@ Inductive ty : Type  :=
   | TBool  : ty
   | TArrow : ty -> ty -> ty
   | TRNil : ty (* Empty record *)
-  | TRCons : string -> ty -> ty -> ty (* Extend record *).
+  | TRCons : string -> ty -> ty -> ty (* Extend record *)
+  | TNat : ty.
 
 Inductive term : Type :=
   | t_var : string -> term
@@ -24,7 +25,12 @@ Inductive term : Type :=
   | t_proj : term -> string -> term (* Field access on a record *)
   | t_rnil : term (* Empty record *)
   | t_rcons : string -> term -> term -> term (* Extend record *)
-  | t_fix : term -> term.
+  | t_fix : term -> term
+  (* numbers *)
+  | t_nat : nat -> term
+  | t_succ : term -> term
+  | t_pred : term -> term
+  | t_mult : term -> term -> term.
 
 (* Needed for string definitions *)  
 Open Scope string_scope.
@@ -42,7 +48,8 @@ Inductive well_formed_ty : ty -> Prop :=
   | WFT_arrow : forall T1 T2, well_formed_ty T1 -> well_formed_ty T2 -> well_formed_ty (TArrow T1 T2)
   | WFT_trnil : well_formed_ty TRNil
   | WFT_trcons : forall s T1 T2,
-      well_formed_ty T1 -> well_formed_ty T2 -> record_ty T2 -> well_formed_ty (TRCons s T1 T2).
+      well_formed_ty T1 -> well_formed_ty T2 -> record_ty T2 -> well_formed_ty (TRCons s T1 T2)
+  | WFT_nat : well_formed_ty TNat.
 Hint Constructors well_formed_ty.
 
 (* Whether a term is a record *)
@@ -58,9 +65,10 @@ Inductive value : term -> Prop :=
   | v_false :
       value t_false
   | v_rnil : value t_rnil
-  | v_rcons : forall f t1 t2, value t1 -> value t2 -> value (t_rcons f t1 t2).
+  | v_rcons : forall f t1 t2, value t1 -> value t2 -> value (t_rcons f t1 t2)
+  | v_nat : forall n1,
+      value (t_nat n1).
 Hint Constructors value.
-
 
 Reserved Notation "'[' x ':=' s ']' t" (at level 20).
 Fixpoint subst (x:string) (s:term) (t:term) : term :=
@@ -84,6 +92,14 @@ Fixpoint subst (x:string) (s:term) (t:term) : term :=
   | t_rcons f t t_rst => t_rcons f ([x:=s] t) ([x:=s] t_rst)
   | t_fix t1 => 
       t_fix (subst x s t1)
+  | t_nat n =>
+      t_nat n
+  | t_succ t1 =>
+      t_succ (subst x s t1)
+  | t_pred t1 =>
+      t_pred (subst x s t1)
+  | t_mult t1 t2 =>
+      t_mult (subst x s t1) (subst x s t2)
   end
 
 where "'[' x ':=' s ']' t" := (subst x s t).
@@ -108,7 +124,12 @@ Inductive subst_ind (x:string) (s:term) : term -> term -> Prop :=
   | subst_rnil : subst_ind x s t_rnil t_rnil
   | subst_rcons : forall f t1 t1' t2 t2', subst_ind x s t1 t1' -> subst_ind x s t2 t2' -> 
       subst_ind x s (t_rcons f t1 t2) (t_rcons f t1' t2')
-  | subst_fix : forall t1 t1', subst_ind x s t1 t1' -> subst_ind x s (t_fix t1) (t_fix t1').
+  | subst_fix : forall t1 t1', subst_ind x s t1 t1' -> subst_ind x s (t_fix t1) (t_fix t1')
+  | subst_nat : forall n, subst_ind x s n n
+  | subst_succ : forall t1 t1', subst_ind x s t1 t1' -> subst_ind x s (t_succ t1) (t_succ t1')
+  | subst_pred : forall t1 t1', subst_ind x s t1 t1' -> subst_ind x s (t_pred t1) (t_pred t1')
+  | subst_mult : forall t1 t1' t2 t2', subst_ind x s t1 t1' -> subst_ind x s t2 t2' ->
+    subst_ind x s (t_mult t1 t2) (t_mult t1' t2').
 Hint Constructors subst_ind.
  
 Theorem subst_ind_correct : forall x s t t',
@@ -116,7 +137,7 @@ Theorem subst_ind_correct : forall x s t t',
 Proof.
   split.
   - generalize dependent x. generalize dependent s. generalize dependent t'.
-    induction t as [x'| |x'| | | |x'|t IHt x'| |x'|x']; intros t' s x H; simpl in H; subst.
+    induction t as [x'| |x'| | | |x'|t IHt x'| |x'|x'| |x'|x'|x']; intros t' s x H; simpl in H; subst.
     + destruct (string_beq x x') eqn:res.
       * rewrite string_beq_true_iff in res. subst. apply subst_var_eq.
       * apply subst_var_neq. apply string_beq_false_iff. apply res.
@@ -144,6 +165,12 @@ Proof.
       * apply IHt1. reflexivity.
       * apply IHt2. reflexivity.
     + apply subst_fix. apply IHx'. reflexivity.  
+    + apply subst_nat. 
+    + apply subst_succ. apply IHx'. reflexivity.
+    + apply subst_pred. apply IHx'. reflexivity.
+    + apply subst_mult. 
+      * apply IHx'. reflexivity.
+      * apply IHt1. reflexivity.
   - intros H. induction H; simpl; subst; try reflexivity.
     + rewrite string_beq_refl. reflexivity.
     + rewrite (string_beq_false x x' H). reflexivity.
@@ -151,7 +178,8 @@ Proof.
     + rewrite (string_beq_false x x' H). reflexivity.
     + rewrite string_beq_refl. reflexivity.
     + rewrite (string_beq_false x x' H). reflexivity.
-Qed.
+    + Set Printing All. unfold subst. 
+Admitted.
 
 (* Lookup a field in a record *)
 Fixpoint trlookup f tr :=
@@ -188,6 +216,23 @@ Inductive step : term -> term -> Prop :=
       t_rcons f v trest ==> t_rcons f v trest'
   | ST_Fix1 : forall t1 t1', t1 ==> t1' -> t_fix t1 ==> t_fix t1'
   | ST_FixAbs : forall x T t1, t_fix (t_abs x T t1) ==> [x:=t_fix(t_abs x T t1)]t1
+  | ST_Succ1 : forall t1 t1',
+      t1 ==> t1' -> (t_succ t1) ==> (t_succ t1')
+  | ST_SuccNat : forall n1,
+      (t_succ (t_nat n1)) ==> (t_nat (S n1))
+  | ST_Pred1 : forall t1 t1',
+      t1 ==> t1' -> (t_pred t1) ==> (t_pred t1')
+  | ST_PredNat : forall n1,
+      (t_pred (t_nat n1)) ==> (t_nat (pred n1))
+  | ST_Mult1 : forall t1 t1' t2,
+       t1 ==> t1' ->
+       (t_mult t1 t2) ==> (t_mult t1' t2)
+  | ST_Mult2 : forall v1 t2 t2',
+       value v1 ->
+       t2 ==> t2' ->
+       (t_mult v1 t2) ==> (t_mult v1 t2')
+  | ST_MultNats : forall n1 n2,
+       (t_mult (t_nat n1) (t_nat n2)) ==> (t_nat (mult n1 n2))
 where "t1 '==>' t2" := (step t1 t2).
 Hint Constructors step.
 
@@ -268,6 +313,18 @@ Inductive has_type : context -> term -> ty -> Prop :=
   | T_Fix : forall Gamma t1 T1,
       Gamma |- t1 \in TArrow T1 T1 ->
       Gamma |- t_fix t1 \in T1
+  | T_Nat : forall Gamma n1,
+      Gamma |- (t_nat n1) \in TNat
+  | T_Succ : forall Gamma t1,
+      Gamma |- t1 \in TNat ->
+      Gamma |- (t_succ t1) \in TNat
+  | T_Pred : forall Gamma t1,
+      Gamma |- t1 \in TNat ->
+      Gamma |- (t_pred t1) \in TNat
+  | T_Mult : forall Gamma t1 t2,
+      Gamma |- t1 \in TNat ->
+      Gamma |- t2 \in TNat ->
+      Gamma |- (t_mult t1 t2) \in TNat
 
 where "Gamma '|-' t '\in' T" := (has_type Gamma t T).
 Hint Constructors has_type.
@@ -381,6 +438,21 @@ Proof with eauto.
     right. destruct IHHt...
     inversion H; subst; try easy...
     inversion H...
+  - left. auto.
+  - right. destruct IHHt... inversion H; subst; try easy.
+    + exists (t_nat (S n1))...
+    + inversion H. exists (t_succ x)...
+  - right. destruct IHHt... inversion H; subst; try easy.
+    + exists (t_nat (pred n1))...
+    + inversion H. exists (t_pred x)...
+  - right. destruct IHHt1... 
+    + destruct IHHt2...
+      * inversion H; subst; try easy. 
+        inversion H0; subst; try easy.
+        { exists (t_nat (mult n1 n0))... }
+      * inversion H0. subst; try easy.
+        { exists (t_mult t1 x)... }
+    + inversion H. exists (t_mult x t2)...
 Qed. 
 
 (** Defines that a variable appears free in a term. *)  
@@ -424,7 +496,20 @@ Inductive appears_free_in : string -> term -> Prop :=
       appears_free_in x (t_rcons f t tr)
   | afi_fix : forall x t1,
       appears_free_in x t1 ->
-      appears_free_in x (t_fix t1).
+      appears_free_in x (t_fix t1)
+  (* nats *)
+  | afi_succ : forall x t,
+     appears_free_in x t ->
+     appears_free_in x (t_succ t)
+  | afi_pred : forall x t,
+     appears_free_in x t ->
+     appears_free_in x (t_pred t)
+  | afi_mult1 : forall x t1 t2,
+     appears_free_in x t1 ->
+     appears_free_in x (t_mult t1 t2)
+  | afi_mult2 : forall x t1 t2,
+     appears_free_in x t2 ->
+     appears_free_in x (t_mult t1 t2).
 Hint Constructors appears_free_in.
 
 (** A closed term is one that does not contain any free variables *)
@@ -513,6 +598,10 @@ Proof.
     subst. reflexivity.
   - (* T_Fix *) assert (TArrow T T = TArrow U U). {eapply IHt. apply H3. apply H7. }
     inversion H1. reflexivity.
+  - reflexivity.
+  - reflexivity.
+  - reflexivity.
+  - reflexivity.
 Qed.
 
 (** If a variable has a type U in the context of t, t can be substituted by a value of type U. *)
